src/LocalsCompCombined.v
@@ -14,266 +14,43 @@ Require
 .
 
 
-
-Definition compile_switch (cu : StackFlatter2.prog_type) : res LocalsSwitch.prog_type :=
-  OK cu
-  @@@ LocalsDestsComp.compile_cu
-  @@ LocalsSwitchComp.compile_cu.
-
-Section FSIMswitch.
-
-  Variable a : StackFlatter2.prog_type.
-  Variable b : LocalsSwitch.prog_type.
-  Hypothesis TRANSF : compile_switch a = OK b.
-
-  Lemma compile_switch_succ :
-    { c | LocalsDestsComp.compile_cu a = Some c }.
-  Proof.
-    unfold compile_switch in TRANSF. break_result_chain. eauto.
-  Qed.
-  
-  Definition fsim_switch : Semantics.forward_simulation (StackFlatter2.semantics a) (LocalsSwitch.semantics b).
-    destruct compile_switch_succ.
-    eapply Semantics.compose_forward_simulation;
-      try eapply LocalsDestsComp.fsim; eauto;
-      try eapply LocalsSwitchComp.fsim; eauto.
-    unfold compile_switch in *; break_result_chain.
-    congruence.
-  Defined.
-
-  Lemma fsim_switch_match_val :
-    forall x y,
-      Semantics.fsim_match_val _ _ fsim_switch x y <-> eq x y.
-  Proof.
-    intros. unfold fsim_switch.
-    destruct compile_switch_succ.
-    erewrite Semantics.fsim_match_val_compose. repeat instantiate (1 := eq).
-    split; intros; repeat break_exists; repeat eexists; repeat break_and; eauto; try congruence.
-    erewrite LocalsDestsComp.match_val_eq.
-    intros; split; intros; congruence.
-    erewrite LocalsSwitchComp.match_val_eq.
-    intros; split; intros; congruence.
-  Qed.    
-
-End FSIMswitch.
-
-Definition compile_return (cu : StackFlatter2.prog_type) : res LocalsReturn.prog_type :=
-  OK cu
-  @@@ compile_switch
-  @@@ LocalsReturnComp.compile_cu.
-
-Section FSIMreturn.
-
-  Variable a : StackFlatter2.prog_type.
-  Variable b : LocalsReturn.prog_type.
-  Hypothesis TRANSF : compile_return a = OK b.
-
-  Lemma compile_return_succ :
-    { c | compile_switch a = Some c }.
-  Proof.
-    unfold compile_return in TRANSF. break_result_chain. eauto.
-  Qed.
-  
-  Definition fsim_return : Semantics.forward_simulation (StackFlatter2.semantics a) (LocalsReturn.semantics b).
-    destruct compile_return_succ.
-    eapply Semantics.compose_forward_simulation;
-      try eapply fsim_switch; eauto;
-      try eapply LocalsReturnComp.fsim; eauto.
-    unfold compile_return in *; break_result_chain.
-    unfold option_to_res in *. congruence.
-  Defined.
-
-  Lemma fsim_return_match_val :
-    forall x y,
-      Semantics.fsim_match_val _ _ fsim_return x y <-> eq x y.
-  Proof.
-    intros. unfold fsim_return.
-    destruct compile_return_succ.
-    erewrite Semantics.fsim_match_val_compose. repeat instantiate (1 := eq).
-    split; intros; repeat break_exists; repeat eexists; repeat break_and; eauto; try congruence.
-    intros. erewrite fsim_switch_match_val.
-    intros; split; intros; congruence.
-    erewrite LocalsReturnComp.match_val_eq.
-    intros; split; intros; congruence.
-  Qed.    
-
-End FSIMreturn.
-
-Definition compile_sources (cu : StackFlatter2.prog_type) : res LocalsSources.prog_type :=
-  OK cu
-  @@@ compile_return
-  @@@ LocalsSourcesComp.compile_cu.
-
-Section FSIMsources.
-
-  Variable a : StackFlatter2.prog_type.
-  Variable b : LocalsSources.prog_type.
-  Hypothesis TRANSF : compile_sources a = OK b.
-
-  Lemma compile_sources_succ :
-    { c | compile_return a = Some c }.
-  Proof.
-    unfold compile_sources in TRANSF. break_result_chain. eauto.
-  Qed.
-  
-  Definition fsim_sources : Semantics.forward_simulation (StackFlatter2.semantics a) (LocalsSources.semantics b).
-    destruct compile_sources_succ.
-    eapply Semantics.compose_forward_simulation;
-      try eapply fsim_return; eauto;
-      try eapply LocalsSourcesComp.fsim; eauto.
-    unfold compile_sources in *; break_result_chain.
-    unfold option_to_res in *. congruence.
-  Defined.
-
-  Lemma fsim_sources_match_val :
-    forall x y,
-      Semantics.fsim_match_val _ _ fsim_sources x y <-> eq x y.
-  Proof.
-    intros. unfold fsim_sources.
-    destruct compile_sources_succ.
-    erewrite Semantics.fsim_match_val_compose. repeat instantiate (1 := eq).
-    split; intros; repeat break_exists; repeat eexists; repeat break_and; eauto; try congruence.
-    intros. erewrite fsim_return_match_val.
-    intros; split; intros; congruence.
-    erewrite LocalsSourcesComp.match_val_eq.
-    intros; split; intros; congruence.
-  Qed.    
-
-End FSIMsources.
-
-
-Definition compile_only (cu : StackFlatter2.prog_type) : res LocalsOnly.prog_type :=
-  OK cu
-  @@@ compile_sources
-  @@ LocalsOnlyComp.compile_cu.
-
-Section FSIMonly.
-
-  Variable a : StackFlatter2.prog_type.
-  Variable b : LocalsOnly.prog_type.
-  Hypothesis TRANSF : compile_only a = OK b.
-
-  Lemma compile_only_succ :
-    { c | compile_sources a = Some c }.
-  Proof.
-    unfold compile_only in TRANSF. break_result_chain. eauto.
-  Qed.
-  
-  Definition fsim_only : Semantics.forward_simulation (StackFlatter2.semantics a) (LocalsOnly.semantics b).
-    destruct compile_only_succ.
-    eapply Semantics.compose_forward_simulation;
-      try eapply fsim_sources; eauto;
-      try eapply LocalsOnlyComp.fsim; eauto.
-    unfold compile_only in *; break_result_chain.
-    unfold option_to_res in *. congruence.
-  Defined.
-
-  Lemma fsim_only_match_val :
-    forall x y,
-      Semantics.fsim_match_val _ _ fsim_only x y <-> eq x y.
-  Proof.
-    intros. unfold fsim_only.
-    destruct compile_only_succ.
-    erewrite Semantics.fsim_match_val_compose. repeat instantiate (1 := eq).
-    split; intros; repeat break_exists; repeat eexists; repeat break_and; eauto; try congruence.
-    intros. erewrite fsim_sources_match_val.
-    intros; split; intros; congruence.
-    erewrite LocalsOnlyComp.match_val_eq.
-    intros; split; intros; congruence.
-  Qed.    
-
-End FSIMonly.
-
-
-
-
 Module A := StackFlatter2.
 Module B := LocalsOnly.
 
-
-Definition compile_cu (cu : A.env * list metadata) : res (B.env * list metadata) := compile_only cu.
+Definition compile_cu (cu : A.prog_type) : res B.prog_type :=
+        OK cu
+    @@@ LocalsDestsComp.compile_cu
+    @@  LocalsSwitchComp.compile_cu
+    @@@ LocalsReturnComp.compile_cu
+    @@@ LocalsSourcesComp.compile_cu
+    @@  LocalsOnlyComp.compile_cu
+.
 
 
 Section Preservation.
 
-  Variable prog : A.prog_type.
-  Variable tprog : B.prog_type.
+Variable aprog : A.prog_type.
+Variable bprog : B.prog_type.
 
-  Hypothesis TRANSF : compile_cu prog = OK tprog.
+Hypothesis Hcomp : compile_cu aprog = OK bprog.
 
+Definition fsim : Semantics.forward_simulation (A.semantics aprog) (B.semantics bprog).
+  unfold compile_cu in Hcomp.
+  break_result_chain.
 
-  Definition fsim : Semantics.forward_simulation (A.semantics prog) (B.semantics tprog).
-    eapply fsim_only. eassumption.
-  Defined.
+  eapply Semantics.compose_forward_simulation. eauto using LocalsDestsComp.fsim.
+  eapply Semantics.compose_forward_simulation. eauto using LocalsSwitchComp.fsim.
+  eapply Semantics.compose_forward_simulation. eauto using LocalsReturnComp.fsim.
+  eapply Semantics.compose_forward_simulation. eauto using LocalsSourcesComp.fsim.
+  eauto using LocalsOnlyComp.fsim.
+Qed.
 
-  Lemma match_val :
-    forall x y,
-      Semantics.fsim_match_val _ _ fsim x y <-> eq x y.
-  Proof.
-    unfold fsim.
-    eapply fsim_only_match_val.
-  Qed.
-  
+Lemma fsim_match_val :
+  forall x y,
+    Semantics.fsim_match_val _ _ fsim x y <-> x = y.
+Proof.
+  intros. erewrite (Semantics.fsim_match_val_canon _ _ fsim).
+  simpl. tauto.
+Qed.
+
 End Preservation.
-
-
-Inductive I : A.state -> B.state -> Prop :=
-| ICombined : forall s00 s01 s02 s03 s04 s05,
-        LocalsDestsComp.I   s00 s01 ->
-        LocalsSwitchComp.I  s01 s02 ->
-        LocalsReturnComp.I  s02 s03 ->
-        LocalsSourcesComp.I s03 s04 ->
-        LocalsOnlyComp.I    s04 s05 ->
-        I s00 s05.
-
-Inductive I_func : list A.insn -> list B.insn * nat -> Prop :=
-| IFuncCombined : forall f00 f01 f02 f03 f04 f05,
-        Forall2 LocalsDestsComp.I_insn      f00 f01 ->
-        Forall2 LocalsSwitchComp.I_insn     f01 f02 ->
-        LocalsReturnComp.I_func             f02 f03 ->
-        LocalsSourcesComp.I_func            f03 f04 ->
-        LocalsOnlyComp.I_func               f04 f05 ->
-        I_func f00 f05.
-
-
-Lemma chain_I_env :
-    forall e00 e01 e02 e03 e04 e05,
-        Forall2 (Forall2 LocalsDestsComp.I_insn)    e00 e01 ->
-        Forall2 (Forall2 LocalsSwitchComp.I_insn)   e01 e02 ->
-        Forall2 (LocalsReturnComp.I_func)           e02 e03 ->
-        Forall2 (LocalsSourcesComp.I_func)          e03 e04 ->
-        Forall2 (LocalsOnlyComp.I_func)             e04 e05 ->
-        Forall2 I_func e00 e05.
-intros.
-list_magic_on (e00, (e01, (e02, (e03, (e04, (e05, tt)))))).
-eapply IFuncCombined; eassumption.
-Qed.
-
-
-
-Theorem compile_I_func : forall a ameta b bmeta,
-    compile_cu (a, ameta) = OK (b, bmeta) ->
-    Forall2 I_func a b.
-intros0 Hcomp. unfold compile_cu in *.
-
-unfold compile_only in *.
-unfold compile_sources in *.
-unfold compile_return in *.
-unfold compile_switch in *.
-
-remember (a, ameta) as aprog.
-break_result_chain.
-subst aprog.  repeat on (_ * _)%type, fun x => destruct x.
-
-on _, eapply_lem LocalsDestsComp.compile_cu_I_env.
-on _, eapply_lem LocalsSwitchComp.compile_cu_I_env.
-on _, eapply_lem LocalsReturnComp.compile_cu_I_env.
-on _, eapply_lem LocalsSourcesComp.compile_cu_I_env.
-on _, eapply_lem LocalsOnlyComp.compile_cu_I_env.
-
-eapply chain_I_env; eassumption.
-Qed.
-
-
-
-
