src/AllValues.v
@@ -1,0 +1,92 @@
+Require HighestValues.
+Require HigherValue.
+Require HighValues.
+
+Require MatchValues.
+
+
+Inductive value_level : Set :=
+| VlHighest
+| VlHigher
+| VlHigh
+.
+
+
+Definition value_type vl : Type :=
+    match vl with
+    | VlHighest => HighestValues.value
+    | VlHigher => HigherValue.value
+    | VlHigh => HighValues.value
+    end.
+
+Definition value_match vl1 vl2 : value_type vl1 -> value_type vl2 -> Prop :=
+    match vl1, vl2 with
+
+    (* zero steps *)
+    | VlHighest, VlHighest => eq
+    | VlHigher, VlHigher => eq
+    | VlHigh, VlHigh => eq
+
+    (* one step *)
+    | VlHighest, VlHigher => MatchValues.mv_higher
+    | VlHigher, VlHigh => MatchValues.mv_high
+
+    (* two steps *)
+    | VlHighest, VlHigh => fun v1 v3 => exists v2,
+            MatchValues.mv_higher v1 v2 /\
+            MatchValues.mv_high v2 v3
+
+    (* anything else *)
+    | _, _ => fun _ _ => False
+    end.
+
+Definition value_level_le vl1 vl2 : Prop :=
+    match vl1, vl2 with
+
+    (* zero steps *)
+    | VlHighest, VlHighest => True
+    | VlHigher, VlHigher => True
+    | VlHigh, VlHigh => True
+
+    (* one step *)
+    | VlHighest, VlHigher => True
+    | VlHigher, VlHigh => True
+
+    (* two steps *)
+    | VlHighest, VlHigh => True
+
+    (* anything else *)
+    | _, _ => False
+    end.
+
+
+Lemma value_match_compose : forall vl1 vl2 vl3 v1 v2 v3,
+    value_match vl1 vl2 v1 v2 ->
+    value_match vl2 vl3 v2 v3 ->
+    value_match vl1 vl3 v1 v3.
+destruct vl1, vl2, vl3; intros ? ? ? Hm1 Hm2; simpl in *; subst;
+solve [eauto | exfalso; eauto | congruence].
+Qed.
+
+Lemma value_match_decompose : forall vl1 vl2 vl3 v1 v3,
+    value_match vl1 vl3 v1 v3 ->
+    value_level_le vl1 vl2 ->
+    value_level_le vl2 vl3 ->
+    exists v2, value_match vl1 vl2 v1 v2 /\ value_match vl2 vl3 v2 v3.
+destruct vl1, vl2, vl3; intros ? ? ? Hle1 Hle2;
+try solve [inversion Hle1 | inversion Hle2];
+simpl in *; eauto.
+Qed.
+
+Lemma value_level_le_refl : forall vl,
+    value_level_le vl vl.
+destruct vl; simpl; eauto.
+Qed.
+
+Lemma value_level_le_trans : forall vl1 vl2 vl3,
+    value_level_le vl1 vl2 ->
+    value_level_le vl2 vl3 ->
+    value_level_le vl1 vl3.
+destruct vl1, vl2, vl3; idtac + exfalso; solve [eauto].
+Qed.
+
