src/SwitchedComp1.v
@@ -492,22 +492,12 @@ Section Preservation.
       eexists. split. 2: reflexivity.
       econstructor; eauto.
 
+    - simpl. eauto.
+    - simpl. intros. tauto.
+
     - intros0 Astep. intros0 II.
       eapply splus_semantics_sim, I_sim; eauto.
 
-    Defined.
-
-    Lemma match_val_eq :
-      Semantics.fsim_match_val _ _ fsim = eq.
-    Proof.
-      unfold fsim. simpl.
-      unfold Semantics.fsim_match_val.
-      break_match. repeat (break_match_hyp; try congruence).
-      try unfold forward_simulation_step in *.
-      try unfold forward_simulation_plus in *.
-      try unfold forward_simulation_star in *.
-      try unfold forward_simulation_star_wf in *.
-      inv Heqf. admit. (*reflexivity.*)
-    Admitted.
+    Qed.
 
 End Preservation.
